theories/zoo/iris/diaframe/diaframe.v
@@ -8,7 +8,23 @@ From zoo.iris Require Export
 From zoo Require Import
   options.
 
-Tactic Notation "iFrameSteps" integer(n) :=
-  do n iFrame; iSteps.
+#[local] Ltac iFrameSteps_ n_frame :=
+  do n_frame iFrame; iSteps.
+Tactic Notation "iFrameSteps" integer(n_frame) :=
+  iFrameSteps_ n_frame.
 Tactic Notation "iFrameSteps" :=
-  iFrameSteps 1.
+  iFrameSteps_ integer:(1).
+
+#[local] Ltac iStepFrameSteps_ n_step n_frame :=
+  let step := ltac2:(n_step |-
+    let opts := parse_iStep_options [] in
+    let n_step := Option.get (Ltac1.to_int n_step) in
+    iStep_num opts n_step
+  ) in
+  step n_step; iFrameSteps_ n_frame.
+Tactic Notation "iStepFrameSteps" integer(n_step) integer(n_frame) :=
+  iStepFrameSteps_ n_step n_frame.
+Tactic Notation "iStepFrameSteps" integer(n_step) :=
+  iStepFrameSteps_ n_step integer:(1).
+Tactic Notation "iStepFrameSteps" :=
+  iStepFrameSteps_ integer:(1) integer:(1).
